RelationalAlgebra/Util/Equiv.lean
@@ -2,8 +2,6 @@ import RelationalAlgebra.RelationalModel
 
 open RM
 
--- Useful helper theorems
-
 -- Allow for deconstructing RelationInstance equivalence into separate schema and tuple equivalence
 @[simp]
 protected theorem RelationInstance.eq.mp : ∀ {a b : RelationInstance α μ}, (a.schema = b.schema ∧ a.tuples = b.tuples) → a = b
@@ -19,19 +17,3 @@ theorem RelationInstance.eq : ∀ {a b : RelationInstance α μ}, (a.schema = b.
 @[simp]
 theorem RelationInstance.dom_eq_schema {r : RelationInstance α μ} {h : t ∈ r.tuples} : t.Dom = r.schema :=
   by rw [RelationInstance.validSchema r t h]
-
-section invFun
-
-variable [Nonempty α] {a : α} {b : β} {f : α → β}
-
-@[simp]
-theorem inv_f_id (h : f.Bijective) : (Function.invFun f ∘ f) a = a
-  := by simp_all only [Function.invFun_comp h.1, id_eq]
-
-@[simp]
-theorem inv_f_id_apply (h : f.Bijective) : Function.invFun f (f a) = a
-  := inv_f_id h
-
-@[simp]
-theorem f_inv_id (h : f.Bijective) : f (Function.invFun f b) = b
-  := by simp_all only [Function.Bijective, Function.Surjective, Function.invFun_eq]
